prove something about mapf_cast

src/Reflection/NamedBase/MapCast.v
@@ -1,27 +1,26 @@
+Require Import Crypto.Util.Tactics Crypto.Util.Option Crypto.Util.Sigma.
 Require Import Coq.Bool.Sumbool.
 Require Import Crypto.Reflection.NamedBase.Syntax.
 
 Local Open Scope nexpr_scope.
 Section language.
   Context {base_type_code : Type}
+          {op : forall t1 t2 tR : base_type_code, Type}
           {Name : Type}
           {interp_base_type_bounds : base_type_code -> Type}
           (interp_op_bounds : forall src1 src2 dst, interp_base_type_bounds src1 -> interp_base_type_bounds src2 -> interp_base_type_bounds dst)
           (pick_typeb : forall t, interp_base_type_bounds t -> base_type_code)
-          (cast_op : forall t1 t2 tR arg1_bs arg2_bs
-                            (arg1v : exprf base_type_code Name (pick_typeb _ arg1_bs))
-                            (arg2v : exprf base_type_code Name (pick_typeb _ arg2_bs)),
-              exprf base_type_code Name (pick_typeb _ (interp_op_bounds t1 t2 tR arg1_bs arg2_bs)))
-          {Context : Context Name interp_base_type_bounds}.
+          (cast_op : forall t1 t2 tR, op t1 t2 tR -> forall arg1_bs arg2_bs, op (pick_typeb _ arg1_bs) (pick_typeb _ arg2_bs) (pick_typeb _ (interp_op_bounds t1 t2 tR arg1_bs arg2_bs)))
+          {BoundsContext : Context Name interp_base_type_bounds}.
 
   Fixpoint mapf_cast
-           (ctx : Context)
-           {t} (e : exprf base_type_code Name t)
+           (ctx : BoundsContext)
+           {t} (e : exprf base_type_code op Name t)
            {struct e}
     : option { bounds : interp_base_type_bounds t
-                        & exprf base_type_code Name (pick_typeb _ bounds) }
-    := match e in exprf _ _ t return option { bounds : interp_base_type_bounds t
-                                                       & exprf base_type_code Name (pick_typeb _ bounds) } with
+                        & exprf base_type_code op Name (pick_typeb _ bounds) }
+    := match e in exprf _ _ _ t return option { bounds : interp_base_type_bounds t
+                                                       & exprf base_type_code op Name (pick_typeb _ bounds) } with
        | Var t x
          => option_map
               (fun bounds => existT _ bounds (Var x))
@@ -35,14 +34,177 @@ Section language.
                    (@mapf_cast (extendb (t:=tx) ctx n x_bounds) _ eC)
             | None => None
             end
-       | BinOp t1 t2 tR arg1 arg2
+       | BinOp t1 t2 tR o arg1 arg2
          => match @mapf_cast ctx _ arg1, @mapf_cast ctx _ arg2 with
             | Some (existT arg1_bounds arg1'),
               Some (existT arg2_bounds arg2')
               => Some (existT _
                               (interp_op_bounds _ _ _ arg1_bounds arg2_bounds)
-                              (cast_op _ _ _ arg1_bounds arg2_bounds arg1' arg2'))
+                              (BinOp (cast_op t1 t2 tR o arg1_bounds arg2_bounds) arg1' arg2'))
             | None, _ | _, None => None
             end
        end.
+
+  Local Arguments interpf {_} {_} {_} {_} {_} {_} _ {_} _.
+  Lemma mapf_cast_correct
+        {interp_base_type : base_type_code -> Type}
+        (interp_op:forall src1 src2 dst : base_type_code,
+            op src1 src2 dst -> interp_base_type src1 -> interp_base_type src2 -> interp_base_type dst)
+        (cast_back: forall t b, interp_base_type (pick_typeb t b) -> interp_base_type t)
+        {Context : Context Name interp_base_type}
+        (inbounds : forall t, interp_base_type_bounds t -> interp_base_type t -> Prop)
+        (interp_op_bounds_correct:
+           forall t1 t2 tR o b1 b2
+             (v1 : interp_base_type t1) (v2 : interp_base_type t2)
+             (H1 : inbounds t1 b1 v1) (H2 : inbounds t2 b2 v2),
+             inbounds tR (interp_op_bounds t1 t2 tR b1 b2) (interp_op t1 t2 tR o v1 v2))
+        (pull_cast_back:
+           forall t1 t2 tR o b1 b2
+             (v1 : interp_base_type (pick_typeb t1 b1)) (v2 : interp_base_type (pick_typeb t2 b2))
+             (H1 : inbounds t1 b1 (cast_back t1 b1 v1)) (H2 : inbounds t2 b2 (cast_back t2 b2 v2)),
+             interp_op t1 t2 tR o (cast_back t1 b1 v1) (cast_back t2 b2 v2)
+             =
+             cast_back _ _ (interp_op _ _ _  (cast_op _ _ _ o b1 b2) v1 v2))
+        {t} (e:exprf base_type_code op Name t)
+    : forall
+        (oldValues:Context)
+        (newValues:Context)
+        (varBounds:BoundsContext)
+        {b} e' (He':mapf_cast varBounds e = Some (existT _ b e'))
+        (Hctx:forall {t} n v,
+            lookupb (t:=t) oldValues n = Some v
+            -> exists b, lookupb (t:=t) varBounds n = Some b
+                         /\ @inbounds _ b v
+                         /\ exists v', lookupb (t:=pick_typeb t b) newValues n = Some v'
+                                       /\ cast_back t b v' = v)
+        r (Hr:interpf (interp_op:=interp_op) oldValues e = Some r)
+        r' (Hr':interpf (interp_op:=interp_op) newValues e' = Some r')
+        , r = cast_back _ _ r' /\ @inbounds _ b r.
+  Proof.
+    induction e; simpl interpf; simpl mapf_cast; unfold option_map; intros;
+      repeat (break_match_hyps; inversion_option; inversion_sigma; simpl in *; subst).
+    { destruct (Hctx _ _ _ Hr) as [b' [Hb'[Hb'v[v'[Hv' Hv'v]]]]]; clear Hctx Hr; subst.
+      repeat match goal with
+               [H: ?e = Some ?x, G:?e = Some ?x' |- _] =>
+               pose proof (eq_trans (eq_sym G) H); clear G; inversion_option; subst
+             end.
+      auto. }
+    { specialize (IHe1 oldValues newValues varBounds _ _ Heqo2 Hctx _ Heqo0 _ Heqo4); clear Heqo2 Heqo0 Heqo4.
+      specialize (IHe2 oldValues newValues varBounds _ _ Heqo3 Hctx _ Heqo1 _ Heqo5); clear Heqo3 Heqo1 Heqo5.
+      destruct_head and; subst; auto. }
+    { admit. }
+  Admitted.
+
 End language.
+
+Require Import ZArith Lia.
+Section example.
+  Inductive base_type_code :=
+  | TZ
+  | TW32
+  | TW64.
+  Inductive op : base_type_code -> base_type_code -> base_type_code -> Type :=
+  | OpMulZ : forall t1 t2, op t1 t2 TZ
+  | OpMul32 : forall t1 t2, op t1 t2 TW32
+  | OpMul64 : forall t1 t2, op t1 t2 TW64.
+  Definition bounds (t:base_type_code) := Z. (* upper bound only for now *)
+  Definition interp_op_bounds (src1 src2 dst : base_type_code) := Z.mul.
+  Definition pick_typeb (t : base_type_code) (b:bounds t) : base_type_code :=
+      match t with
+        | TW32 => TW32
+        | TW64 => if Z.ltb b (2^32) then TW32 else TW64
+        | TZ => 
+          if Z.ltb b (2^32) then TW32
+          else if Z.ltb b (2^64) then TW64
+               else TZ
+      end.
+
+  Definition cast_op (t1 t2 tR : base_type_code) (o:op t1 t2 tR) (arg1_bs : bounds t1) (arg2_bs : bounds t2)
+    : op (pick_typeb t1 arg1_bs) (pick_typeb t2 arg2_bs)
+         (pick_typeb tR (interp_op_bounds t1 t2 tR arg1_bs arg2_bs)) :=
+    match pick_typeb tR (interp_op_bounds t1 t2 tR arg1_bs arg2_bs) with
+    | TZ => OpMulZ _ _
+    | TW32 => OpMul32 _ _
+    | TW64 => OpMul64 _ _
+    end.
+
+  Definition interp_base_type t :=
+    match t with
+    | TZ => Z
+    | TW32 => { z | (Z.leb 0 z && Z.ltb z (2^32)%Z = true)%bool }
+    | TW64 => { z | (Z.leb 0 z && Z.ltb z (2^64)%Z = true)%bool }
+    end.
+  Check @mapf_cast_correct base_type_code op positive bounds interp_op_bounds pick_typeb cast_op
+        _ (* ctx *)
+        interp_base_type.
+
+  Definition to_Z {t:base_type_code} : interp_base_type t -> Z :=
+    match t with
+    | TZ => fun v => v
+    | _ => fun v => proj1_sig v
+    end.
+
+  Definition of_Z (t:base_type_code) (v:Z) : interp_base_type t. refine
+    match t as t return interp_base_type t with
+    | TZ => v
+    | TW32 => exist _ (v mod 2^32)%Z _
+    | TW64 => exist _ (v mod 2^64)%Z _
+    end; abstract(rewrite !Bool.andb_true_iff, !Z.leb_le, Z.ltb_lt; apply Z_mod_lt; reflexivity). Defined.
+      
+  Definition cast_back (t : base_type_code) (b : bounds t) (v:interp_base_type (pick_typeb t b))
+    : interp_base_type t := of_Z _ (to_Z v).
+
+  Definition interp_op (src1 src2 dst : base_type_code) (o:op src1 src2 dst)
+             (x:interp_base_type src1) (y:interp_base_type src2) : interp_base_type dst :=
+    of_Z _ (Z.mul (to_Z x) (to_Z y)).
+
+  Definition inbounds t (b:bounds t) (v:interp_base_type t)
+    := (0 <= to_Z v < b)%Z.
+
+  Lemma interp_op_bounds_correct t1 t2 tR o b1 b2
+        (v1 : interp_base_type t1) (v2 : interp_base_type t2)
+        (H1 : @inbounds t1 b1 v1) (H2 : @inbounds t2 b2 v2)
+    : inbounds tR (interp_op_bounds t1 t2 tR b1 b2) (interp_op t1 t2 tR o v1 v2).
+  Proof.
+    destruct o; cbv [inbounds interp_op_bounds interp_op] in *;
+      generalize dependent (to_Z v1); generalize dependent (to_Z v2);
+        clear dependent v1; clear dependent v2;
+          intros z1 H1 z2 H2; cbv [of_Z to_Z id proj1_sig] in *.
+    { cbv [of_Z to_Z id] in *. nia. }
+    admit.
+    admit.
+  Admitted.
+
+  Local Arguments Z.pow : simpl never.
+  Lemma to_Z_cast_back t (b:bounds t) (v:interp_base_type (pick_typeb t b))
+    : to_Z (cast_back t b v) = to_Z v.
+  Proof.
+    destruct t;
+      repeat (trivial;
+              rewrite ?Bool.andb_true_iff, ?Z.leb_le, ?Z.ltb_lt in *; 
+              cbv [cast_back]; break_match; simpl in *;
+              destruct_head' sig;
+              rewrite ?Zmod_small by nia).
+  Qed.
+
+  Require Import Decidable.
+  Lemma pull_cast_back t1 t2 tR o b1 b2
+        (v1 : interp_base_type (pick_typeb t1 b1)) (v2 : interp_base_type (pick_typeb t2 b2))
+        (H1 : inbounds t1 b1 (cast_back t1 b1 v1)) (H2 : inbounds t2 b2 (cast_back t2 b2 v2))
+  : interp_op t1 t2 tR o (cast_back t1 b1 v1) (cast_back t2 b2 v2)
+  = cast_back _ _ (interp_op _ _ _  (cast_op _ _ _ o b1 b2) v1 v2).
+  Proof.
+    cbv [inbounds interp_op_bounds interp_op] in *.
+    cbv [cast_back pick_typeb]; break_match; simpl;
+      rewrite ?to_Z_cast_back, ?Decidable.eqsig_eq, ?Zmod_small; trivial;
+        rewrite ?Bool.andb_true_iff, ?Z.leb_le, ?Z.ltb_lt in *.
+  Admitted.
+
+  Check @mapf_cast_correct base_type_code op positive bounds interp_op_bounds pick_typeb cast_op
+        _ (* ctx *)
+        interp_base_type interp_op cast_back
+        _ (* ctx *)
+        inbounds
+        interp_op_bounds_correct
+        pull_cast_back
+        .
